BooleanSemantics.v
@@ -1,0 +1,287 @@
+Require Import List Lia.
+Import ListNotations.
+
+Require Import Regex Chars Groups.
+Require Import Tree.
+Require Import Semantics.
+
+(** * Loop Boolean  *)
+(* The loop boolean, indicating if we can exit a loop iteration or not *)
+(* CanExit means that we are allowed to exit any quantifier: we have read a character more recently than we have entered a free quantifier *)
+(* CannotExit means we can't exit the most recent quantifier we entered, because we haven't read anything since *)
+Inductive LoopBool : Type :=
+| CanExit
+| CannotExit.
+
+
+(** * Boolean Semantics  *)
+(* where checks consult the boolean instead of actually comparing strings *)
+
+Inductive bool_tree: regex -> continuation -> input -> LoopBool -> tree -> Prop :=
+| bool_epsilon:
+  (* on an empty continuation *)
+  forall inp b,
+    bool_tree Epsilon [] inp b (Match inp)
+| bool_pop_reg:
+  (* pops a regex from the continuation list *)
+  forall inp regcont tailcont treecont b
+    (TREECONT: bool_tree regcont tailcont inp b treecont),
+    bool_tree Epsilon (Areg regcont :: tailcont) inp b treecont
+| bool_pop_check:
+  (* pops a successful check from the continuation list *)
+  (* this only checks the boolean allows exit and not the strcheck in the tree *)
+  forall inp strcheck tailcont treecont
+    (TREECONT: bool_tree Epsilon tailcont inp CanExit treecont),
+    bool_tree Epsilon (Acheck strcheck :: tailcont) inp CanExit (CheckPass strcheck treecont)
+| bool_pop_check_fail:
+  (* pops a failing check from the continuation list *)
+  (* this require the boolean to disallow exit *)
+  forall inp strcheck tailcont,
+    bool_tree Epsilon (Acheck strcheck :: tailcont) inp CannotExit (CheckFail strcheck)
+| bool_pop_close:
+(* pops the closing of a group from the continuation list *)
+  forall inp tailcont treecont gid b
+    (TREECONT: bool_tree Epsilon tailcont inp b treecont),
+    bool_tree Epsilon (Aclose gid :: tailcont) inp b (CloseGroup gid treecont)
+| bool_char:
+  (* changes the boolean so that we can now exit *)
+  forall c cd inp nextinp cont tcont b
+    (READ: read_char cd inp = Some (c, nextinp))
+    (TREECONT: bool_tree Epsilon cont nextinp CanExit tcont),
+    bool_tree (Character cd) cont inp b (Read c tcont)
+| bool_char_fail:
+  forall cd inp cont b
+    (READ: read_char cd inp = None),
+    bool_tree (Character cd) cont inp b Mismatch
+| bool_disj:
+  forall r1 r2 cont t1 t2 inp b
+    (ISTREE1: bool_tree r1 cont inp b t1)
+    (ISTREE2: bool_tree r2 cont inp b t2),
+    bool_tree (Disjunction r1 r2) cont inp b (Choice t1 t2)
+| bool_sequence:
+  (* adding next regex to the continuation *)
+  forall r1 r2 cont t inp b
+    (CONT: bool_tree r1 (Areg r2 :: cont) inp b t),
+    bool_tree (Sequence r1 r2) cont inp b t
+| bool_star:
+  forall r1 cont titer tskip tquant inp gidl b
+    (* the list of capture groups to reset *)
+    (RESET: gidl = def_groups r1)
+    (* doing one iteration, then a check, then executing the next quantifier *)
+    (* switching the boolean such that we can't exit right away *)
+    (ISTREE1: bool_tree r1 (Acheck (current_str inp)::Areg (Star r1)::cont) inp CannotExit titer)
+    (* skipping the star entirely *)
+    (SKIP: bool_tree Epsilon cont inp b tskip)
+    (CHOICE: tquant = Choice (ResetGroups gidl titer) tskip),
+    bool_tree (Star r1) cont inp b tquant
+| bool_group:
+  forall r1 cont treecont inp gid b
+    (TREECONT: bool_tree r1 (Aclose gid :: cont) inp b treecont),
+    bool_tree (Group gid r1) cont inp b (OpenGroup gid treecont).
+
+
+(** * Boolean Tree Equivalence  *)
+
+(* As we go down the tree, the boolean should "encode" the continuation and the current string *)
+(* Meaning that the boolean is true when we can exit with the current string *)
+(* And the boolean is false when we cannot *)
+
+
+(** * First Step: encoding the invariant  *)
+Definition suffix (str1 str2:string) : Prop :=
+  exists prefix, str2 = prefix ++ str1.
+
+Definition strict_suffix (str1 str2:string) : Prop :=
+  suffix str1 str2 /\ str1 <> str2.
+
+Lemma cons_neq:
+  forall A str pref (c:A),
+    str = pref ++ c::str -> False.
+Proof.
+  intros A str pref c H.
+  assert (List.length str = List.length pref + 1 + List.length str).
+  { rewrite H at 1. rewrite app_length. simpl. lia. }
+  lia.
+Qed.
+
+Lemma strict_cons:
+  forall s c,
+    strict_suffix s (c::s).
+Proof.
+  intros s c. unfold strict_suffix, suffix. split.
+  - exists [c]. simpl. auto.
+  - unfold not.
+    replace (c::s) with ([] ++ c::s) by auto.
+    apply cons_neq.
+Qed.    
+
+Lemma strict_app:
+  forall str1 str2 c,
+    strict_suffix (c::str1) str2 ->
+    strict_suffix str1 str2.
+Proof.
+  unfold strict_suffix, suffix. intros str2 str0 c [[prefix APP] NEQ].
+  split.
+  - exists (prefix ++ [c]). rewrite <- app_assoc. simpl. auto.
+  - unfold not. intros H. subst. eapply cons_neq; eauto.
+Qed.
+  
+
+Inductive bool_encoding: LoopBool -> string -> continuation -> Prop :=
+(* with an empty continuation we can be encoded with any boolean *)
+| nil_encode:
+  forall str b,
+    bool_encoding b str []
+| cons_reg:
+  forall b str cont r
+    (ENCODE: bool_encoding b str cont),
+    bool_encoding b str (Areg r::cont)
+| cons_close:
+  forall b str cont gid
+    (ENCODE: bool_encoding b str cont),
+    bool_encoding b str (Aclose gid::cont)
+| cons_true:
+  forall stk str head 
+    (ENCODE: bool_encoding CanExit str stk)
+    (STRICT: strict_suffix str head),
+    bool_encoding CanExit str (Acheck head::stk)
+| to_false:
+  (* to switch to false, we need the head of the stack to be equal to the current string
+   no progress has been made. *)
+  forall stk str
+    (ENCODE: bool_encoding CanExit str stk),
+    bool_encoding CannotExit str (Acheck str::stk)
+| cons_false:
+  (* when the bool is already false, we can push the current string to the stack *)
+  forall stk str
+    (ENCODE: bool_encoding CannotExit str stk),
+    bool_encoding CannotExit str (Acheck str::stk).
+
+(* Generalizes the encoding to inputs *)
+(* later: add direction, so that the input can be read in two directions *)
+Inductive encodes : LoopBool -> input -> continuation -> Prop :=
+| encode_forward:
+  forall b next pref cont
+    (ENCODE: bool_encoding b next cont),
+    encodes b (Input next pref) cont.
+
+
+(* when we are already encoded with true, reading a new character preserves this true encoding *)
+(* when we are encoded with false, reading a new character switches to being encoded with true *)
+Lemma true_encoding:
+  forall str c cont b,
+    bool_encoding b (c::str) cont ->
+    bool_encoding CanExit str cont.
+Proof.
+  intros str c cont b H.
+  remember (c::str) as prevstr.
+  induction H; intros.
+  - constructor.
+  - constructor; auto.
+  - constructor; auto.
+  - constructor; auto. rewrite Heqprevstr in STRICT. eapply strict_app; eauto.
+  - constructor.
+    + apply IHbool_encoding; auto.
+    + rewrite Heqprevstr. apply strict_cons.
+  - constructor.
+    + apply IHbool_encoding; auto.
+    + rewrite Heqprevstr. apply strict_cons.
+Qed.
+
+
+(* when entering a new quantifier, this pushes the current string on the stack *)
+(* this makes the whole stack encoded with false *)
+Lemma false_encoding:
+  forall str cont b,
+    bool_encoding b str cont ->
+    bool_encoding CannotExit str (Acheck str::cont).
+Proof.
+  intros str cont b H.
+  induction H.
+  - constructor. constructor.
+  - inversion IHbool_encoding; subst.
+    + apply to_false. constructor. auto.
+    + apply cons_false. constructor. auto.
+  - inversion IHbool_encoding; subst.
+    + apply to_false. constructor. auto.
+    + apply cons_false. constructor. auto.
+  - apply to_false. apply cons_true; auto.
+  - apply cons_false. auto.
+  - apply cons_false. auto.
+Qed.
+
+(* if the string is different than the check, we know the boolean is true *)
+Lemma encoding_different:
+  forall b str strcheck cont,
+    bool_encoding b str (Acheck strcheck::cont) ->
+    str <> strcheck ->
+    b = CanExit.
+Proof.
+  intros b0 str strcheck cont H.
+  remember (Acheck strcheck::cont) as prevcont.
+  induction H; intros; auto; inversion Heqprevcont;
+    exfalso; auto.
+Qed.
+
+(* if the check is going to fail, we know the boolean is false *)
+Lemma encoding_same:
+  forall b str cont,
+    bool_encoding b str (Acheck str::cont) -> b = CannotExit.
+Proof.
+  intros b str cont H.
+  remember (Acheck str::cont) as prevcont.
+  induction H; intros; auto; inversion Heqprevcont.
+  subst. destruct STRICT as [_ NEQ].
+  exfalso. apply NEQ. auto.
+Qed.
+
+(** * Second Step: encoding equality  *)
+(* the two tree constructions are equal *)
+
+Theorem encode_equal:
+  forall r inp cont b t
+    (ENCODE: encodes b inp cont)
+    (TREE: is_tree r cont inp t),
+    bool_tree r cont inp b t.
+Proof.
+  intros r inp cont b0 t ENCODE TREE.
+  generalize dependent b0.
+  induction TREE; intros.
+  - constructor.
+  - constructor.
+    eapply IHTREE; eauto.
+    inversion ENCODE; subst; constructor; inversion ENCODE0; auto.
+  - assert (b0 = CanExit).
+    { remember (Acheck strcheck::tailcont) as cont'.
+      destruct ENCODE; subst; eapply encoding_different; eauto. }
+    subst. constructor. eapply IHTREE; eauto.
+    inversion ENCODE; subst; constructor; inversion ENCODE0; auto.
+  - assert (b0 = CannotExit).
+    { remember (Acheck strcheck :: tailcont) as cont'.
+      destruct ENCODE; subst; eapply encoding_same; eauto. }
+    subst. constructor.
+  - constructor. apply IHTREE.
+    inversion ENCODE; subst; constructor; inversion ENCODE0; auto.
+  - econstructor; eauto. apply IHTREE.
+    destruct nextinp. destruct ENCODE; constructor; simpl in READ.
+    destruct next0; inversion READ. destruct (char_match c0 cd); inversion READ; subst. eapply true_encoding; eauto.
+  - constructor; auto.
+  - constructor; auto.
+  - constructor. apply IHTREE; eauto.
+    inversion ENCODE; subst; constructor; constructor; auto.
+  - eapply bool_star; eauto.
+    apply IHTREE1.
+    destruct ENCODE; constructor; simpl; eapply false_encoding; constructor; eauto.
+  - constructor. apply IHTREE.
+    destruct ENCODE; constructor; constructor; auto.
+Qed.
+    
+Corollary boolean_correct:
+  forall r str t,
+    backtree r str t ->
+    bool_tree r [] (init_input str) CanExit t.
+Proof.
+  unfold backtree. intros r str t H.
+  eapply encode_equal; eauto.
+  constructor. constructor.
+Qed.
